Proofs/Form.thy
@@ -60,21 +60,4 @@ fun wf_logic_node_inputs :: "IRGraph \<Rightarrow> ID \<Rightarrow> bool" where
 "wf_logic_node_inputs g n =
   (\<forall> inp \<in> set (inputs_of (kind g n)) . (\<forall> v m p . ([g, m, p] \<turnstile> kind g inp \<mapsto> v) \<longrightarrow> wf_bool v))"
 
-fun wf_values :: "IRGraph \<Rightarrow> bool" where
-  "wf_values g = (\<forall> n \<in> ids g .
-    (\<forall> v m p . ([g, m, p] \<turnstile> kind g n \<mapsto> v) \<longrightarrow> 
-      (wf_value v \<and> 
-      (is_LogicNode (kind g n) \<longrightarrow> 
-        wf_bool v \<and> wf_logic_node_inputs g n))))"
-
-lemma wf_value_range:
-  "b > 1 \<and> b \<in> int_bits_allowed \<longrightarrow> {v. wf_value (IntVal b v)} = {v. ((-(2^(b-1)) \<le> v) \<and> (v < (2^(b-1))))}"
-  unfolding wf_value.simps
-  by auto
-
-lemma wf_value_bit_range:
-  "b = 1 \<longrightarrow> {v. wf_value (IntVal b v)} = {}"
-  unfolding wf_value.simps
-  by (simp add: int_bits_allowed_def)
-
 end
